# baseURI: http:semanticweb.org/hohfeldiansystem/

@prefix : <http:semanticweb.org/hohfeldiansystem/> .
@prefix AllCoreOntology: <http://www.ontologyrepository.com/CommonCoreOntologies/Mid/AllCoreOntology#> .
@prefix ROImport: <http://www.ontologyrepository.com/CommonCoreOntologies/Upper/ROImport#> .
@prefix obo: <http://purl.obolibrary.org/obo/> .
@prefix owl: <http://www.w3.org/2002/07/owl#> .
@prefix rdf: <http://www.w3.org/1999/02/22-rdf-syntax-ns#> .
@prefix rdfs: <http://www.w3.org/2000/01/rdf-schema#> .
@prefix skos: <http://www.w3.org/2004/02/skos/core#> .
@prefix terms: <http://purl.org/dc/terms/> .
@prefix xml: <http://www.w3.org/XML/1998/namespace> .
@prefix xsd: <http://www.w3.org/2001/XMLSchema#> .


:
  rdf:type owl:Ontology ;
  terms:creator "J. Neil Otte" ;
  rdfs:comment "This ontology models The Hohfeldian System of Rights. The four basic components of rights are known as “the Hohfeldian incidents” after Wesley Hohfeld (1879–1918), the American legal theorist who discovered them. The four atomic rights include the privilege, the claim, the power, and the immunity."@en ;
  rdfs:label "Hohfeldian Rights Ontology"@en ;
.
:rights_0000001
  rdf:type rdfs:Resource ;
  rdf:type owl:Class ;
  terms:bibliographicCitation "Wenar, Leif, \"Rights\", The Stanford Encyclopedia of Philosophy (Spring 2020 Edition), Edward N. Zalta (ed.), URL = <https://plato.stanford.edu/archives/spr2020/entries/rights/>" ;
  rdfs:label "Right"@en ;
  owl:disjointWith :rights_0000012 ;
  skos:definition "A defined class equivalent to Atomic Right or Molecular Right."@en ;
.
:rights_0000002
  rdf:type rdfs:Resource ;
  rdf:type owl:Class ;
  terms:bibliographicCitation "Wenar, Leif, \"Rights\", The Stanford Encyclopedia of Philosophy (Spring 2020 Edition), Edward N. Zalta (ed.), URL = <https://plato.stanford.edu/archives/spr2020/entries/rights/>" ;
  rdfs:label "Atomic Right"@en ;
  rdfs:subClassOf :rights_0000001 ;
  owl:disjointWith :rights_0000003 ;
  owl:equivalentClass [
      rdf:type owl:Class ;
      owl:unionOf (
          :rights_0000008
          :rights_0000009
          :rights_0000010
          :rights_0000011
        ) ;
    ] ;
  skos:definition "A defined class equivalent to an instance of a power, privilege, liberty, or immunity."@en ;
.
:rights_0000003
  rdf:type rdfs:Resource ;
  rdf:type owl:Class ;
  terms:bibliographicCitation "Wenar, Leif, \"Rights\", The Stanford Encyclopedia of Philosophy (Spring 2020 Edition), Edward N. Zalta (ed.), URL = <https://plato.stanford.edu/archives/spr2020/entries/rights/> " ;
  rdfs:label "Molecular Right"@en ;
  rdfs:subClassOf :rights_0000001 ;
  owl:equivalentClass [
      rdf:type owl:Class ;
      owl:intersectionOf (
          :rights_0000001
          [
            rdf:type owl:Class ;
            owl:unionOf (
                [
                  rdf:type owl:Class ;
                  owl:intersectionOf (
                      [
                        rdf:type owl:Restriction ;
                        owl:onProperty obo:BFO_0000051 ;
                        owl:someValuesFrom :rights_0000008 ;
                      ]
                      [
                        rdf:type owl:Restriction ;
                        owl:onProperty obo:BFO_0000051 ;
                        owl:someValuesFrom :rights_0000009 ;
                      ]
                    ) ;
                ]
                [
                  rdf:type owl:Class ;
                  owl:intersectionOf (
                      [
                        rdf:type owl:Restriction ;
                        owl:onProperty obo:BFO_0000051 ;
                        owl:someValuesFrom :rights_0000008 ;
                      ]
                      [
                        rdf:type owl:Restriction ;
                        owl:onProperty obo:BFO_0000051 ;
                        owl:someValuesFrom :rights_0000009 ;
                      ]
                      [
                        rdf:type owl:Restriction ;
                        owl:onProperty obo:BFO_0000051 ;
                        owl:someValuesFrom :rights_0000010 ;
                      ]
                    ) ;
                ]
                [
                  rdf:type owl:Class ;
                  owl:intersectionOf (
                      [
                        rdf:type owl:Restriction ;
                        owl:onProperty obo:BFO_0000051 ;
                        owl:someValuesFrom :rights_0000008 ;
                      ]
                      [
                        rdf:type owl:Restriction ;
                        owl:onProperty obo:BFO_0000051 ;
                        owl:someValuesFrom :rights_0000009 ;
                      ]
                      [
                        rdf:type owl:Restriction ;
                        owl:onProperty obo:BFO_0000051 ;
                        owl:someValuesFrom :rights_0000010 ;
                      ]
                      [
                        rdf:type owl:Restriction ;
                        owl:onProperty obo:BFO_0000051 ;
                        owl:someValuesFrom :rights_0000011 ;
                      ]
                    ) ;
                ]
                [
                  rdf:type owl:Class ;
                  owl:intersectionOf (
                      [
                        rdf:type owl:Restriction ;
                        owl:onProperty obo:BFO_0000051 ;
                        owl:someValuesFrom :rights_0000008 ;
                      ]
                      [
                        rdf:type owl:Restriction ;
                        owl:onProperty obo:BFO_0000051 ;
                        owl:someValuesFrom :rights_0000009 ;
                      ]
                      [
                        rdf:type owl:Restriction ;
                        owl:onProperty obo:BFO_0000051 ;
                        owl:someValuesFrom :rights_0000011 ;
                      ]
                    ) ;
                ]
                [
                  rdf:type owl:Class ;
                  owl:intersectionOf (
                      [
                        rdf:type owl:Restriction ;
                        owl:onProperty obo:BFO_0000051 ;
                        owl:someValuesFrom :rights_0000008 ;
                      ]
                      [
                        rdf:type owl:Restriction ;
                        owl:onProperty obo:BFO_0000051 ;
                        owl:someValuesFrom :rights_0000010 ;
                      ]
                    ) ;
                ]
                [
                  rdf:type owl:Class ;
                  owl:intersectionOf (
                      [
                        rdf:type owl:Restriction ;
                        owl:onProperty obo:BFO_0000051 ;
                        owl:someValuesFrom :rights_0000008 ;
                      ]
                      [
                        rdf:type owl:Restriction ;
                        owl:onProperty obo:BFO_0000051 ;
                        owl:someValuesFrom :rights_0000010 ;
                      ]
                      [
                        rdf:type owl:Restriction ;
                        owl:onProperty obo:BFO_0000051 ;
                        owl:someValuesFrom :rights_0000011 ;
                      ]
                    ) ;
                ]
                [
                  rdf:type owl:Class ;
                  owl:intersectionOf (
                      [
                        rdf:type owl:Restriction ;
                        owl:onProperty obo:BFO_0000051 ;
                        owl:someValuesFrom :rights_0000008 ;
                      ]
                      [
                        rdf:type owl:Restriction ;
                        owl:onProperty obo:BFO_0000051 ;
                        owl:someValuesFrom :rights_0000011 ;
                      ]
                    ) ;
                ]
                [
                  rdf:type owl:Class ;
                  owl:intersectionOf (
                      [
                        rdf:type owl:Restriction ;
                        owl:onProperty obo:BFO_0000051 ;
                        owl:someValuesFrom :rights_0000009 ;
                      ]
                      [
                        rdf:type owl:Restriction ;
                        owl:onProperty obo:BFO_0000051 ;
                        owl:someValuesFrom :rights_0000010 ;
                      ]
                    ) ;
                ]
                [
                  rdf:type owl:Class ;
                  owl:intersectionOf (
                      [
                        rdf:type owl:Restriction ;
                        owl:onProperty obo:BFO_0000051 ;
                        owl:someValuesFrom :rights_0000009 ;
                      ]
                      [
                        rdf:type owl:Restriction ;
                        owl:onProperty obo:BFO_0000051 ;
                        owl:someValuesFrom :rights_0000010 ;
                      ]
                      [
                        rdf:type owl:Restriction ;
                        owl:onProperty obo:BFO_0000051 ;
                        owl:someValuesFrom :rights_0000011 ;
                      ]
                    ) ;
                ]
                [
                  rdf:type owl:Class ;
                  owl:intersectionOf (
                      [
                        rdf:type owl:Restriction ;
                        owl:onProperty obo:BFO_0000051 ;
                        owl:someValuesFrom :rights_0000009 ;
                      ]
                      [
                        rdf:type owl:Restriction ;
                        owl:onProperty obo:BFO_0000051 ;
                        owl:someValuesFrom :rights_0000011 ;
                      ]
                    ) ;
                ]
                [
                  rdf:type owl:Class ;
                  owl:intersectionOf (
                      [
                        rdf:type owl:Restriction ;
                        owl:onProperty obo:BFO_0000051 ;
                        owl:someValuesFrom :rights_0000010 ;
                      ]
                      [
                        rdf:type owl:Restriction ;
                        owl:onProperty obo:BFO_0000051 ;
                        owl:someValuesFrom :rights_0000011 ;
                      ]
                    ) ;
                ]
              ) ;
          ]
        ) ;
    ] ;
  skos:definition "A rule that consists of an aggregate of one or more privileges, powers, liberties, or immunities."@en ;
.
:rights_0000004
  rdf:type rdfs:Resource ;
  rdf:type owl:Class ;
  terms:bibliographicCitation "Wenar, Leif, \"Rights\", The Stanford Encyclopedia of Philosophy (Spring 2020 Edition), Edward N. Zalta (ed.), URL = <https://plato.stanford.edu/archives/spr2020/entries/rights/>" ;
  rdfs:label "Primary Rule"@en ;
  rdfs:subClassOf :rights_0000002 ;
  owl:disjointWith :rights_0000005 ;
  owl:equivalentClass [
      rdf:type owl:Class ;
      owl:unionOf (
          :rights_0000008
          :rights_0000010
        ) ;
    ] ;
  skos:definition "A rule requiring that people perform or refrain from performing particular actions (Hart 1961). Indeed the primary rules for all physical actions are properly analyzed as privileges and claims. Were we to know all privileges and claims concerning physical actions, we would know for every possible physical action whether that action was permitted, required, or forbidden."@en ;
.
:rights_0000005
  rdf:type rdfs:Resource ;
  rdf:type owl:Class ;
  terms:bibliographicCitation "Wenar, Leif, \"Rights\", The Stanford Encyclopedia of Philosophy (Spring 2020 Edition), Edward N. Zalta (ed.), URL = <https://plato.stanford.edu/archives/spr2020/entries/rights/>" ;
  rdfs:label "Secondary Rule"@en ;
  rdfs:subClassOf :rights_0000002 ;
  owl:equivalentClass [
      rdf:type owl:Class ;
      owl:unionOf (
          :rights_0000009
          :rights_0000011
        ) ;
    ] ;
  skos:definition "A rule that specifies how agents can introduce and change primary rules."@en ;
.
:rights_0000006
  rdf:type rdfs:Resource ;
  rdf:type owl:Class ;
  terms:bibliographicCitation "Wenar, Leif, \"Rights\", The Stanford Encyclopedia of Philosophy (Spring 2020 Edition), Edward N. Zalta (ed.), URL = <https://plato.stanford.edu/archives/spr2020/entries/rights/>" ;
  rdfs:label "Active Right"@en ;
  rdfs:subClassOf :rights_0000001 ;
  owl:equivalentClass [
      rdf:type owl:Class ;
      owl:unionOf (
          :rights_0000008
          :rights_0000009
        ) ;
    ] ;
  skos:definition "A right that the bearer has to perform some action."@en ;
.
:rights_0000007
  rdf:type rdfs:Resource ;
  rdf:type owl:Class ;
  terms:bibliographicCitation "Wenar, Leif, \"Rights\", The Stanford Encyclopedia of Philosophy (Spring 2020 Edition), Edward N. Zalta (ed.), URL = <https://plato.stanford.edu/archives/spr2020/entries/rights/>" ;
  rdfs:label "Passive Right"@en ;
  rdfs:subClassOf :rights_0000001 ;
  owl:equivalentClass [
      rdf:type owl:Class ;
      owl:unionOf (
          :rights_0000010
          :rights_0000011
        ) ;
    ] ;
  skos:definition "A right that bearer has that another agent perform some action."@en ;
.
:rights_0000008
  rdf:type rdfs:Resource ;
  rdf:type owl:Class ;
  terms:bibliographicCitation "Wenar, Leif, \"Rights\", The Stanford Encyclopedia of Philosophy (Spring 2020 Edition), Edward N. Zalta (ed.), URL = <https://plato.stanford.edu/archives/spr2020/entries/rights/>" ;
  rdfs:comment "Axiom: A has a privilege to ɸ if and only if A has no duty not to ɸ. Axiom: If A has a privilege that Aɸ, then A has no duty that not A ɸ."@en ;
  rdfs:label "Privilege"@en ;
  rdfs:subClassOf :rights_0000004 ;
  owl:disjointWith :rights_0000009 ;
  owl:disjointWith :rights_0000010 ;
  owl:disjointWith :rights_0000011 ;
  skos:altlabel "Liberty"@en ;
  skos:definition "A primary rule where the subject may perform an action and has no duty not to perform the action"@en ;
  skos:example "You have a right to pick up a shell that you find on the beach."@en ;
.
:rights_0000009
  rdf:type rdfs:Resource ;
  rdf:type owl:Class ;
  terms:bibliographicCitation "Wenar, Leif, \"Rights\", The Stanford Encyclopedia of Philosophy (Spring 2020 Edition), Edward N. Zalta (ed.), URL = <https://plato.stanford.edu/archives/spr2020/entries/rights/>" ;
  rdfs:comment "Axiom: A has a power if and only if A has the ability to alter her own or another's Hohfeldian incidents."@en ;
  rdfs:label "Power"@en ;
  rdfs:subClassOf :rights_0000005 ;
  owl:disjointWith :rights_0000010 ;
  owl:disjointWith :rights_0000011 ;
  skos:altlabel "Ability"@en ;
  skos:definition "A secondary rule that allows the subject to alter an incident of themselves or another"@en ;
  skos:example "A ship's captain has the power-right to order a midshipman to scrub the deck. Ordering, promising, waiving, abandoning, consenting, selling, and sentencing are all examples of acts by which a rightholder exercises a power to change his own Hohfeldian incidents or those of another."@en ;
.
:rights_0000010
  rdf:type rdfs:Resource ;
  rdf:type owl:Class ;
  terms:bibliographicCitation "Wenar, Leif, \"Rights\", The Stanford Encyclopedia of Philosophy (Spring 2020 Edition), Edward N. Zalta (ed.), URL = <https://plato.stanford.edu/archives/spr2020/entries/rights/>" ;
  rdfs:comment "Axiom: A has a claim that B ɸ if and only if B has a duty to A to ɸ."@en ;
  rdfs:label "Claim"@en ;
  rdfs:subClassOf :rights_0000004 ;
  owl:disjointWith :rights_0000011 ;
  skos:definition "A primary rule that always mutually depends upon a duty in another individual that is owed to the subject"@en ;
  skos:example "A contract between employer and employee confers on the employee a right to be paid her wages."@en ;
.
:rights_0000011
  rdf:type rdfs:Resource ;
  rdf:type owl:Class ;
  terms:bibliographicCitation "Wenar, Leif, \"Rights\", The Stanford Encyclopedia of Philosophy (Spring 2020 Edition), Edward N. Zalta (ed.), URL = <https://plato.stanford.edu/archives/spr2020/entries/rights/>" ;
  rdfs:comment """Axiom: B has an immunity if and only if A lacks the ability to alter B's Hohfeldian incidents.
Axioms: When A has the ability to alter B's Hohfeldian incidents, then A has a power. When A lacks the ability to alter B's Hohfeldian incidents, then B has an immunity."""@en ;
  rdfs:label "Immunity"@en ;
  rdfs:subClassOf :rights_0000005 ;
  skos:definition "A secondary rule where the subject of an incident cannot have the incident altered by the ability of another"@en ;
  skos:example "Example: The United States Congress lacks the ability within the Constitution to impose upon American citizens a duty to kneel daily before a cross. Since the Congress lacks a power, the citizens have an immunity."@en ;
.
:rights_0000012
  rdf:type rdfs:Resource ;
  rdf:type owl:Class ;
  terms:bibliographicCitation "Wenar, Leif, \"Rights\", The Stanford Encyclopedia of Philosophy (Spring 2020 Edition), Edward N. Zalta (ed.), URL = <https://plato.stanford.edu/archives/spr2020/entries/rights/>" ;
  rdfs:label "Duty"@en ;
  skos:altlabel "Obligation"@en ;
  skos:definition "A rule whose subject owes, is obliged, or is required to perform some action"@en ;
.
